src/library/tactic/dsimplify_tactic.h
@@ -4,3 +4,8 @@ Released under Apache 2.0 license as described in the file LICENSE.
 
 Author: Leonardo de Moura
 */
+#pragma once
+namespace lean {
+void initialize_dsimplify_tactic();
+void finalize_dsimplify_tactic();
+}
