tests/lean/run/dsimplify1.lean
@@ -1,0 +1,17 @@
+open tactic
+
+example (f : nat → nat → nat) (p : nat → Prop) (a b : nat) : f ((a + 1, b).1) b = f (a+1) (a, b).2 :=
+by do
+  t ← target,
+  new_t ← dsimplify (λ e, failed) (λ e, do new_e ← whnf e, return (new_e, tt)) t,
+  expected ← to_expr `(f (nat.succ a) b = f (nat.succ a) b),
+  guard (new_t = expected),
+  reflexivity
+
+example (f : nat → nat → nat) (p : nat → Prop) (a b : nat) : f ((a + 1, b).1) b = f (a+1) (a, b).2 :=
+by do
+  t ← target,
+  new_t ← dsimplify (λ e, failed) (λ e, do new_e ← whnf_no_delta e, return (new_e, tt)) t,
+  expected ← to_expr `(f (a + 1) b = f (a + 1) b),
+  guard (new_t = expected),
+  reflexivity
